src/SDK/Serialize.dfy
@@ -142,7 +142,7 @@ module Serialize {
 
     // Serialization is easier to implement and verify by first converting the map to
     // a sequence of pairs.
-    var keys : seq<UTF8.ValidUTF8Bytes> := Sets.ComputeSetToOrderedSequence(encryptionContext.Keys, UInt.UInt8Less);
+    var keys: seq<UTF8.ValidUTF8Bytes> := Sets.ComputeSetToOrderedSequence(encryptionContext.Keys, UInt.UInt8Less);
     var kvPairs := seq(|keys|, i requires 0 <= i < |keys| => (keys[i], encryptionContext[keys[i]]));
 
     var j := 0;
